Turned off auto-implicits and added initial Total semantics to Annotated syntax

Total/Stlc/Lang/Annotated/Semantics.lean
@@ -25,4 +25,66 @@ namespace Total.Stlc.Lang.Annotated
     inductive Eval₁ (ρ: Ty → Type) (τ: Ty): Top ρ τ → Top ρ τ → Prop where
     def Eval (ρ: Ty → Type) (τ: Ty) := RTC (Eval₁ ρ τ)
   end Top
+
+  namespace PrimOp
+    @[reducible]
+    def Halts {ρ: Ty → Type} (τ: Ty) (p: PrimOp) (t₁: Term ρ τ): Prop := ∃ t₂: Term ρ τ, Eval₁ p t₁ t₂ ∧ Term.IsValue t₂
+
+    @[reducible]
+    def Total {ρ: Ty → Type} (τ₁ τ₂: Ty) (op: UnOp) (t: Term ρ): Prop :=
+      (HasType op τ₁ τ₂) ∧ (Halts op t) ∧ True
+
+    namespace Total
+      theorem halts {τ₁ τ₂: Ty} {op: UnOp} {t: Term}: Total τ₁ τ₂ op t → Halts op t
+        | ⟨_, hh, _⟩ => hh
+    end Total
+  end PrimOp
+
+  namespace Term
+    @[reducible]
+    def Halts {ρ: Ty → Type} {τ: Ty} (t₁: Term ρ τ): Prop := ∃ t₂: Term ρ τ, Eval ρ τ t₁ t₂ ∧ IsValue ρ τ t₂
+
+    @[reducible]
+    def Total {ρ: Ty → Type} (τ: Ty) (t: Term ρ τ): Prop :=
+      (Halts t) ∧ (
+        match τ with
+          | .bool => True
+          | .nat  => True
+          | .fn _ _ => sorry
+      )
+
+    namespace IsValue
+      theorem halts {ρ: Ty → Type} {τ: Ty} {t: Term ρ τ}: IsValue ρ τ t → Halts t
+        | .bool _ => ⟨_, .refl, .bool _⟩
+        | .nat  _ => ⟨_, .refl, .nat  _⟩
+    end IsValue
+
+    namespace Total
+      theorem halts {ρ: Ty → Type} {τ: Ty}: {t: Term ρ τ} → Total τ t → Halts t
+        | .bool _, _ => IsValue.halts (.bool _)
+        | .nat _,  _ => IsValue.halts (.nat  _)
+
+        | .primOp _, _ => sorry
+
+        | .cond _ _ _,  ⟨_, ⟨_, he, hv⟩, _⟩ => ⟨_, he, hv⟩
+    end Total
+  end Term
+
+  namespace Top
+    @[reducible]
+    def Halts {ρ: Ty → Type} {τ: Ty} (t₁: Top ρ τ): Prop := ∃ t₂: Top ρ τ, Eval ρ τ t₁ t₂ ∧ IsValue ρ τ t₂
+
+    @[reducible]
+    def Total {ρ: Ty → Type} {τ: Ty}: Ty → Top ρ τ → Prop
+      | .bool, t => nomatch t
+
+    namespace IsValue
+      theorem halts {ρ: Ty → Type} {τ: Ty} {t: Top ρ τ}: IsValue ρ τ t → Halts t := nomatch t
+    end IsValue
+
+    namespace Total
+      theorem halts {ρ: Ty → Type} {τ: Ty} {t: Top ρ τ}: Top ρ τ → Halts t
+        | t => nomatch t
+    end Total
+  end Top
 end Total.Stlc.Lang.Annotated
